@prefix dbr: <http://dbpedia.org/page/> .
@prefix dct: <http://purl.org/dc/terms/> .
@prefix foaf: <http://xmlns.com/foaf/0.1/> .
@prefix owl: <http://www.w3.org/2002/07/owl#> .
@prefix rdfs: <http://www.w3.org/2000/01/rdf-schema#> .
@prefix skos: <http://www.w3.org/2004/02/skos/core#> .
@prefix swift: <http://purl.org/lu/uni/alma/swift#> .

<http://purl.org/lu/uni/alma/swift> a owl:Ontology ;
    dct:created "2020-04-27" ;
    dct:creator [ a foaf:Person ;
            foaf:mbox <christian.grevisse@uni.lu> ;
            foaf:name "Christian GREVISSE" ] ;
    dct:description "This is an SKOS-based vocabulary about the Swift programming language." ;
    dct:license <https://creativecommons.org/licenses/by-sa/4.0/> ;
    dct:modified "2020-04-27" ;
    dct:subject dbr:Swift_%28programming_language%29 ;
    dct:title "Swift Vocabulary" ;
    rdfs:seeAlso <https://coast.uni.lu/alma/> ;
    owl:imports <http://www.w3.org/2004/02/skos/core> ;
    owl:versionIRI <http://purl.org/lu/uni/alma/swift/5.2> ;
    owl:versionInfo "5.2/1.0.0" .

swift:Any a owl:NamedIndividual,
        skos:Concept ;
    skos:broader swift:Type ;
    skos:definition <https://docs.swift.org/swift-book/LanguageGuide/TypeCasting.html#ID342> ;
    skos:inScheme swift:Scheme ;
    skos:prefLabel "Any"@en ;
    skos:related swift:TypeCasting .

swift:AnyObject a owl:NamedIndividual,
        skos:Concept ;
    skos:broader swift:Type ;
    skos:definition <https://docs.swift.org/swift-book/LanguageGuide/TypeCasting.html#ID342> ;
    skos:inScheme swift:Scheme ;
    skos:prefLabel "AnyObject"@en ;
    skos:related swift:Class,
        swift:TypeCasting .

swift:ArgumentLabel a owl:NamedIndividual,
        skos:Concept ;
    skos:definition <https://docs.swift.org/swift-book/LanguageGuide/Functions.html#ID166> ;
    skos:inScheme swift:Scheme ;
    skos:prefLabel "Argument Label"@en ;
    skos:related swift:Parameter .

swift:ArithmeticOperator a owl:NamedIndividual,
        skos:Concept ;
    skos:broader swift:Operator ;
    skos:definition <https://docs.swift.org/swift-book/LanguageGuide/BasicOperators.html#ID63> ;
    skos:inScheme swift:Scheme ;
    skos:prefLabel "Arithmetic Operator"@en ;
    skos:related dbr:Operator_%28computer_programming%29 .

swift:Array a owl:NamedIndividual,
        skos:Concept ;
    skos:broader swift:Collection ;
    skos:definition <https://docs.swift.org/swift-book/LanguageGuide/CollectionTypes.html#ID107> ;
    skos:inScheme swift:Scheme ;
    skos:prefLabel "Array"@en ;
    skos:related dbr:Array_data_type .

swift:AssociatedType a owl:NamedIndividual,
        skos:Concept ;
    skos:definition <https://docs.swift.org/swift-book/LanguageGuide/Generics.html#ID189> ;
    skos:inScheme swift:Scheme ;
    skos:prefLabel "Associated Type"@en ;
    skos:related swift:GenericType,
        swift:Protocol .

swift:AssociatedValue a owl:NamedIndividual,
        skos:Concept ;
    skos:definition <https://docs.swift.org/swift-book/LanguageGuide/Enumerations.html#ID148> ;
    skos:inScheme swift:Scheme ;
    skos:prefLabel "Associated Value"@en ;
    skos:related swift:Enumeration .

swift:Attribute a owl:NamedIndividual,
        skos:Concept ;
    skos:definition <https://docs.swift.org/swift-book/ReferenceManual/Attributes.html#attributes> ;
    skos:inScheme swift:Scheme ;
    skos:prefLabel "Attribute"@en ;
    skos:related dbr:Attribute_%28computing%29 .

swift:Autoclosure a owl:NamedIndividual,
        skos:Concept ;
    skos:broader swift:Closure ;
    skos:definition <https://docs.swift.org/swift-book/LanguageGuide/Closures.html#ID543> ;
    skos:inScheme swift:Scheme ;
    skos:prefLabel "Autoclosure"@en .

swift:BitwiseOperator a owl:NamedIndividual,
        skos:Concept ;
    skos:broader swift:Operator ;
    skos:definition <https://docs.swift.org/swift-book/LanguageGuide/AdvancedOperators.html#ID29> ;
    skos:inScheme swift:Scheme ;
    skos:prefLabel "Bitwise Operator"@en ;
    skos:related dbr:Bitwise_operation .

swift:Bool a owl:NamedIndividual,
        skos:Concept ;
    skos:broader swift:Struct ;
    skos:definition <https://docs.swift.org/swift-book/LanguageGuide/TheBasics.html#ID328> ;
    skos:inScheme swift:Scheme ;
    skos:prefLabel "Boolean"@en ;
    skos:related dbr:Boolean_data_type .

swift:ClosureExpression a owl:NamedIndividual,
        skos:Concept ;
    skos:broader swift:Closure ;
    skos:definition <https://docs.swift.org/swift-book/LanguageGuide/Closures.html#ID95> ;
    skos:inScheme swift:Scheme ;
    skos:prefLabel "Closure Expression"@en .

swift:Comment a owl:NamedIndividual,
        skos:Concept ;
    skos:definition <https://docs.swift.org/swift-book/LanguageGuide/TheBasics.html#ID315> ;
    skos:inScheme swift:Scheme ;
    skos:prefLabel "Comment"@en ;
    skos:related dbr:Comment_%28computer_programming%29 .

swift:ComparisonOperator a owl:NamedIndividual,
        skos:Concept ;
    skos:broader swift:Operator ;
    skos:definition <https://docs.swift.org/swift-book/LanguageGuide/BasicOperators.html#ID70> ;
    skos:inScheme swift:Scheme ;
    skos:prefLabel "Comparison Operator"@en ;
    skos:related dbr:Relational_operator .

swift:CompilerControlStatement a owl:NamedIndividual,
        skos:Concept ;
    skos:definition <https://docs.swift.org/swift-book/ReferenceManual/Statements.html#ID538> ;
    skos:inScheme swift:Scheme ;
    skos:prefLabel "Compiler Control Statement"@en ;
    skos:related dbr:Directive_%28programming%29,
        swift:If .

swift:CompoundAssignmentOperator a owl:NamedIndividual,
        skos:Concept ;
    skos:broader swift:AssignmentOperator ;
    skos:definition <https://docs.swift.org/swift-book/LanguageGuide/AdvancedOperators.html#ID44> ;
    skos:inScheme swift:Scheme ;
    skos:prefLabel "Compound Assignment Operator"@en ;
    skos:related dbr:Augmented_assignment .

swift:CustomOperator a owl:NamedIndividual,
        skos:Concept ;
    skos:broader swift:Operator ;
    skos:definition <https://docs.swift.org/swift-book/LanguageGuide/AdvancedOperators.html#ID46> ;
    skos:inScheme swift:Scheme ;
    skos:prefLabel "Custom Operator"@en .

swift:DefaultInitializer a owl:NamedIndividual,
        skos:Concept ;
    skos:broader swift:Initializer ;
    skos:definition <https://docs.swift.org/swift-book/LanguageGuide/Initialization.html#ID213> ;
    skos:inScheme swift:Scheme ;
    skos:prefLabel "Default Initializer"@en ;
    skos:related dbr:Default_constructor .

swift:DefaultParameterValue a owl:NamedIndividual,
        skos:Concept ;
    skos:definition <https://docs.swift.org/swift-book/LanguageGuide/Functions.html#ID169> ;
    skos:inScheme swift:Scheme ;
    skos:prefLabel "Default Parameter Value"@en ;
    skos:related dbr:Default_argument,
        swift:Parameter .

swift:DefaultPropertyValue a owl:NamedIndividual,
        skos:Concept ;
    skos:definition <https://docs.swift.org/swift-book/LanguageGuide/Initialization.html#ID206> ;
    skos:inScheme swift:Scheme ;
    skos:prefLabel "Default Property Value"@en ;
    skos:related swift:Initializer,
        swift:Property .

swift:DesignatedInitializer a owl:NamedIndividual,
        skos:Concept ;
    skos:broader swift:Initializer ;
    skos:definition <https://docs.swift.org/swift-book/LanguageGuide/Initialization.html#ID217> ;
    skos:inScheme swift:Scheme ;
    skos:prefLabel "Designated Initializer"@en .

swift:Dictionary a owl:NamedIndividual,
        skos:Concept ;
    skos:broader swift:Collection ;
    skos:definition <https://docs.swift.org/swift-book/LanguageGuide/CollectionTypes.html#ID113> ;
    skos:inScheme swift:Scheme ;
    skos:prefLabel "Dictionary"@en ;
    skos:related dbr:Associative_array .

swift:Double a owl:NamedIndividual,
        skos:Concept ;
    skos:broader swift:Struct ;
    skos:definition <https://docs.swift.org/swift-book/LanguageGuide/TheBasics.html#ID321> ;
    skos:inScheme swift:Scheme ;
    skos:prefLabel "Double"@en ;
    skos:related dbr:Double-precision_floating-point_format .

swift:EscapingClosure a owl:NamedIndividual,
        skos:Concept ;
    skos:broader swift:Closure ;
    skos:definition <https://docs.swift.org/swift-book/LanguageGuide/Closures.html#ID546> ;
    skos:inScheme swift:Scheme ;
    skos:prefLabel "Escaping Closure"@en .

swift:FailableInitializer a owl:NamedIndividual,
        skos:Concept ;
    skos:broader swift:Initializer ;
    skos:definition <https://docs.swift.org/swift-book/LanguageGuide/Initialization.html#ID224> ;
    skos:inScheme swift:Scheme ;
    skos:prefLabel "Failable Initializer"@en .

swift:Float a owl:NamedIndividual,
        skos:Concept ;
    skos:broader swift:Struct ;
    skos:definition <https://docs.swift.org/swift-book/LanguageGuide/TheBasics.html#ID321> ;
    skos:inScheme swift:Scheme ;
    skos:prefLabel "Float"@en ;
    skos:related dbr:Floating-point_arithmetic .

swift:ForInLoop a owl:NamedIndividual,
        skos:Concept ;
    skos:broader swift:Loop ;
    skos:definition <https://docs.swift.org/swift-book/LanguageGuide/ControlFlow.html#ID121> ;
    skos:inScheme swift:Scheme ;
    skos:prefLabel "For-In Loop"@en ;
    skos:related dbr:Foreach_loop .

swift:ForcedUnwrapping a owl:NamedIndividual,
        skos:Concept ;
    skos:definition <https://docs.swift.org/swift-book/LanguageGuide/TheBasics.html#ID332> ;
    skos:inScheme swift:Scheme ;
    skos:prefLabel "Forced Unwrapping"@en ;
    skos:related swift:Optional .

swift:FunctionType a owl:NamedIndividual,
        skos:Concept ;
    skos:broader swift:Type ;
    skos:definition <https://docs.swift.org/swift-book/LanguageGuide/Functions.html#ID174> ;
    skos:inScheme swift:Scheme ;
    skos:prefLabel "Function Type"@en ;
    skos:related dbr:Function_type,
        swift:Function .

swift:GenericFunction a owl:NamedIndividual,
        skos:Concept ;
    skos:broader swift:Function ;
    skos:definition <https://docs.swift.org/swift-book/LanguageGuide/Generics.html#ID181> ;
    skos:inScheme swift:Scheme ;
    skos:prefLabel "Generic Function"@en ;
    skos:related dbr:Generic_function,
        swift:Generics .

swift:Guard a owl:NamedIndividual,
        skos:Concept ;
    skos:broader swift:ConditionalStatement ;
    skos:definition <https://docs.swift.org/swift-book/LanguageGuide/ControlFlow.html#ID525> ;
    skos:inScheme swift:Scheme ;
    skos:prefLabel "guard Statement"@en ;
    skos:related dbr:Guard_%28computer_science%29 .

swift:IdentityOperator a owl:NamedIndividual,
        skos:Concept ;
    skos:broader swift:Operator ;
    skos:definition <https://docs.swift.org/swift-book/LanguageGuide/ClassesAndStructures.html#ID90> ;
    skos:inScheme swift:Scheme ;
    skos:prefLabel "Identity Operator"@en ;
    skos:related swift:ReferenceType .

swift:InitializerDelegation a owl:NamedIndividual,
        skos:Concept ;
    skos:definition <https://docs.swift.org/swift-book/LanguageGuide/Initialization.html#ID215> ;
    skos:inScheme swift:Scheme ;
    skos:prefLabel "Initializer Delegation"@en ;
    skos:related swift:Initializer .

swift:InitializerRequirement a owl:NamedIndividual,
        skos:Concept ;
    skos:definition <https://docs.swift.org/swift-book/LanguageGuide/Protocols.html#ID272> ;
    skos:inScheme swift:Scheme ;
    skos:prefLabel "Initializer Requirement"@en ;
    skos:related swift:Initializer,
        swift:Protocol .

swift:InstanceMethod a owl:NamedIndividual,
        skos:Concept ;
    skos:broader swift:Method ;
    skos:definition <https://docs.swift.org/swift-book/LanguageGuide/Methods.html#ID235> ;
    skos:inScheme swift:Scheme ;
    skos:prefLabel "Instance Method"@en .

swift:Int a owl:NamedIndividual,
        skos:Concept ;
    skos:broader swift:Struct ;
    skos:definition <https://docs.swift.org/swift-book/LanguageGuide/TheBasics.html#ID317> ;
    skos:inScheme swift:Scheme ;
    skos:prefLabel "Int"@en ;
    skos:related dbr:Integer_%28computer_science%29 .

swift:LabeledStatement a owl:NamedIndividual,
        skos:Concept ;
    skos:broader swift:ControlFlow ;
    skos:definition <https://docs.swift.org/swift-book/LanguageGuide/ControlFlow.html#ID141> ;
    skos:inScheme swift:Scheme ;
    skos:prefLabel "Labeled Statement"@en ;
    skos:related dbr:Label_%28computer_science%29,
        swift:break,
        swift:continue .

swift:LazyStoredProperty a owl:NamedIndividual,
        skos:Concept ;
    skos:broader swift:StoredProperty ;
    skos:definition <https://docs.swift.org/swift-book/LanguageGuide/Properties.html#ID257> ;
    skos:inScheme swift:Scheme ;
    skos:prefLabel "Lazy Stored Property"@en .

swift:LogicalOperator a owl:NamedIndividual,
        skos:Concept ;
    skos:broader swift:Operator ;
    skos:definition <https://docs.swift.org/swift-book/LanguageGuide/BasicOperators.html#ID76> ;
    skos:inScheme swift:Scheme ;
    skos:prefLabel "Logical Operator"@en ;
    skos:related dbr:Operator_%28computer_programming%29 .

swift:NestedFunction a owl:NamedIndividual,
        skos:Concept ;
    skos:broader swift:Function ;
    skos:definition <https://docs.swift.org/swift-book/LanguageGuide/Functions.html#ID178> ;
    skos:inScheme swift:Scheme ;
    skos:prefLabel "Nested Function"@en ;
    skos:related dbr:Nested_function .

swift:NestedType a owl:NamedIndividual,
        skos:Concept ;
    skos:broader swift:Type ;
    skos:definition <https://docs.swift.org/swift-book/LanguageGuide/NestedTypes.html#nested-types> ;
    skos:inScheme swift:Scheme ;
    skos:prefLabel "Nested Type"@en .

swift:NilCoalescingOperator a owl:NamedIndividual,
        skos:Concept ;
    skos:broader swift:Operator ;
    skos:definition <https://docs.swift.org/swift-book/LanguageGuide/BasicOperators.html#ID72> ;
    skos:inScheme swift:Scheme ;
    skos:prefLabel "Nil-Coalescing Operator"@en ;
    skos:related dbr:Null_coalescing_operator,
        swift:Optional .

swift:OpenAccess a owl:NamedIndividual,
        skos:Concept ;
    skos:broader swift:AccessLevel ;
    skos:inScheme swift:Scheme ;
    skos:prefLabel "Open Access"@en .

swift:OptionalBinding a owl:NamedIndividual,
        skos:Concept ;
    skos:definition <https://docs.swift.org/swift-book/LanguageGuide/TheBasics.html#ID333> ;
    skos:inScheme swift:Scheme ;
    skos:prefLabel "Optional Binding"@en ;
    skos:related swift:If,
        swift:Optional .

swift:OptionalChaining a owl:NamedIndividual,
        skos:Concept ;
    skos:definition <https://docs.swift.org/swift-book/LanguageGuide/OptionalChaining.html> ;
    skos:inScheme swift:Scheme ;
    skos:prefLabel "Optional Chaining"@en ;
    skos:related dbr:Optional_chaining_operator,
        swift:Optional .

swift:OptionalProtocolRequirement a owl:NamedIndividual,
        skos:Concept ;
    skos:definition <https://docs.swift.org/swift-book/LanguageGuide/Protocols.html#ID284> ;
    skos:inScheme swift:Scheme ;
    skos:prefLabel "Optional Protocol Requirement"@en ;
    skos:related swift:MethodRequirement,
        swift:PropertyRequirement,
        swift:Protocol .

swift:OverflowOperator a owl:NamedIndividual,
        skos:Concept ;
    skos:broader swift:Operator ;
    skos:definition <https://docs.swift.org/swift-book/LanguageGuide/AdvancedOperators.html#ID37> ;
    skos:inScheme swift:Scheme ;
    skos:prefLabel "Overflow Operator"@en .

swift:PropertyObserver a owl:NamedIndividual,
        skos:Concept ;
    skos:definition <https://docs.swift.org/swift-book/LanguageGuide/Properties.html#ID262> ;
    skos:inScheme swift:Scheme ;
    skos:prefLabel "Property Observer"@en ;
    skos:related swift:Property .

swift:PropertyWrapper a owl:NamedIndividual,
        skos:Concept ;
    skos:definition <https://docs.swift.org/swift-book/LanguageGuide/Properties.html#ID617> ;
    skos:inScheme swift:Scheme ;
    skos:prefLabel "Property Wrapper"@en ;
    skos:related swift:Property .

swift:ProtocolExtension a owl:NamedIndividual,
        skos:Concept ;
    skos:broader swift:Extension ;
    skos:definition <https://docs.swift.org/swift-book/LanguageGuide/Protocols.html#ID521> ;
    skos:inScheme swift:Scheme ;
    skos:prefLabel "Protocol Extension"@en ;
    skos:related dbr:Trait_%28computer_programming%29,
        swift:Protocol .

swift:RangeOperator a owl:NamedIndividual,
        skos:Concept ;
    skos:broader swift:Operator ;
    skos:definition <https://docs.swift.org/swift-book/LanguageGuide/BasicOperators.html#ID73> ;
    skos:inScheme swift:Scheme ;
    skos:prefLabel "Range Operator"@en ;
    skos:related dbr:Range_%28computer_programming%29 .

swift:RawValue a owl:NamedIndividual,
        skos:Concept ;
    skos:definition <https://docs.swift.org/swift-book/LanguageGuide/Enumerations.html#ID149> ;
    skos:inScheme swift:Scheme ;
    skos:prefLabel "Raw Value"@en ;
    skos:related swift:Enumeration .

swift:RecursiveEnumeration a owl:NamedIndividual,
        skos:Concept ;
    skos:broader swift:Enumeration ;
    skos:definition <https://docs.swift.org/swift-book/LanguageGuide/Enumerations.html#ID536> ;
    skos:inScheme swift:Scheme ;
    skos:prefLabel "Recursive Enumeration"@en .

swift:RepeatWhileLoop a owl:NamedIndividual,
        skos:Concept ;
    skos:broader swift:Loop ;
    skos:definition <https://docs.swift.org/swift-book/LanguageGuide/ControlFlow.html#ID126> ;
    skos:inScheme swift:Scheme ;
    skos:prefLabel "Repeat-While Loop"@en ;
    skos:related dbr:Do_while_loop .

swift:Set a owl:NamedIndividual,
        skos:Concept ;
    skos:broader swift:Collection ;
    skos:definition <https://docs.swift.org/swift-book/LanguageGuide/CollectionTypes.html#ID484> ;
    skos:inScheme swift:Scheme ;
    skos:prefLabel "Set"@en ;
    skos:related dbr:Set_%28abstract_data_type%29 .

swift:StringInterpolation a owl:NamedIndividual,
        skos:Concept ;
    skos:definition <https://docs.swift.org/swift-book/LanguageGuide/StringsAndCharacters.html#ID292> ;
    skos:inScheme swift:Scheme ;
    skos:prefLabel "String Interpolation"@en ;
    skos:related dbr:String_interpolation,
        swift:String .

swift:StrongReference a owl:NamedIndividual,
        skos:Concept ;
    skos:definition <https://docs.swift.org/swift-book/LanguageGuide/AutomaticReferenceCounting.html#ID49> ;
    skos:inScheme swift:Scheme ;
    skos:prefLabel "Strong Reference"@en ;
    skos:related swift:ARC .

swift:Subclassing a owl:NamedIndividual,
        skos:Concept ;
    skos:definition <https://docs.swift.org/swift-book/LanguageGuide/Inheritance.html#ID195> ;
    skos:inScheme swift:Scheme ;
    skos:prefLabel "Subclassing"@en ;
    skos:related dbr:Subclass_%28computer_science%29,
        swift:Inheritance .

swift:TernaryConditionalOperator a owl:NamedIndividual,
        skos:Concept ;
    skos:broader swift:Operator ;
    skos:definition <https://docs.swift.org/swift-book/LanguageGuide/BasicOperators.html#ID71> ;
    skos:inScheme swift:Scheme ;
    skos:prefLabel "Ternary Conditional Operator"@en ;
    skos:related dbr:Elvis_operator,
        dbr:Ternary_operation .

swift:TrailingClosure a owl:NamedIndividual,
        skos:Concept ;
    skos:broader swift:Closure ;
    skos:definition <https://docs.swift.org/swift-book/LanguageGuide/Closures.html#ID102> ;
    skos:inScheme swift:Scheme ;
    skos:prefLabel "Trailing Closure"@en .

swift:Tuple a owl:NamedIndividual,
        skos:Concept ;
    skos:broader swift:ValueType ;
    skos:definition <https://docs.swift.org/swift-book/LanguageGuide/TheBasics.html#ID329> ;
    skos:inScheme swift:Scheme ;
    skos:prefLabel "Tuple"@en ;
    skos:related dbr:Tuple .

swift:TypeAlias a owl:NamedIndividual,
        skos:Concept ;
    skos:definition <https://docs.swift.org/swift-book/LanguageGuide/TheBasics.html#ID327> ;
    skos:inScheme swift:Scheme ;
    skos:prefLabel "Type Alias"@en ;
    skos:related dbr:Typedef,
        swift:Type .

swift:TypeAnnotation a owl:NamedIndividual,
        skos:Concept ;
    skos:definition <https://docs.swift.org/swift-book/LanguageGuide/TheBasics.html#ID312> ;
    skos:inScheme swift:Scheme ;
    skos:prefLabel "Type Annotation"@en ;
    skos:related swift:Type .

swift:TypeCastOperator a owl:NamedIndividual,
        skos:Concept ;
    skos:broader swift:DownCasting,
        swift:Operator ;
    skos:inScheme swift:Scheme ;
    skos:prefLabel "Type Cast Operator"@en .

swift:TypeInference a owl:NamedIndividual,
        skos:Concept ;
    skos:definition <https://docs.swift.org/swift-book/LanguageGuide/TheBasics.html#ID322> ;
    skos:inScheme swift:Scheme ;
    skos:prefLabel "Type Inference"@en ;
    skos:related dbr:Type_inference,
        swift:Type .

swift:TypeMethod a owl:NamedIndividual,
        skos:Concept ;
    skos:broader swift:Method ;
    skos:definition <https://docs.swift.org/swift-book/LanguageGuide/Methods.html#ID241> ;
    skos:inScheme swift:Scheme ;
    skos:prefLabel "Type Method"@en .

swift:TypeParameter a owl:NamedIndividual,
        skos:Concept ;
    skos:broader swift:Parameter ;
    skos:definition <https://docs.swift.org/swift-book/LanguageGuide/Generics.html#ID182> ;
    skos:inScheme swift:Scheme ;
    skos:prefLabel "Type Parameter"@en ;
    skos:related dbr:TypeParameter,
        swift:GenericType .

swift:TypeProperty a owl:NamedIndividual,
        skos:Concept ;
    skos:broader swift:Property ;
    skos:definition <https://docs.swift.org/swift-book/LanguageGuide/Properties.html#ID264> ;
    skos:inScheme swift:Scheme ;
    skos:prefLabel "Type Property"@en ;
    skos:related dbr:Class_variable .

swift:TypeSubscript a owl:NamedIndividual,
        skos:Concept ;
    skos:broader swift:Subscript ;
    skos:definition <https://docs.swift.org/swift-book/LanguageGuide/Subscripts.html#ID609> ;
    skos:inScheme swift:Scheme ;
    skos:prefLabel "Type Subscript"@en .

swift:VariadicParameter a owl:NamedIndividual,
        skos:Concept ;
    skos:broader swift:Parameter ;
    skos:definition <https://docs.swift.org/swift-book/LanguageGuide/Functions.html#ID171> ;
    skos:inScheme swift:Scheme ;
    skos:prefLabel "Variadic Parameter"@en ;
    skos:related dbr:Variadic_function .

swift:WhileLoop a owl:NamedIndividual,
        skos:Concept ;
    skos:broader swift:Loop ;
    skos:definition <https://docs.swift.org/swift-book/LanguageGuide/ControlFlow.html#ID124> ;
    skos:inScheme swift:Scheme ;
    skos:prefLabel "While Loop"@en ;
    skos:related dbr:While_loop .

swift:case a owl:NamedIndividual,
        skos:Concept ;
    skos:broader swift:Keyword ;
    skos:inScheme swift:Scheme ;
    skos:prefLabel "case"@en ;
    skos:related swift:Enumeration,
        swift:Switch .

swift:catch a owl:NamedIndividual,
        skos:Concept ;
    skos:broader swift:Keyword ;
    skos:inScheme swift:Scheme ;
    skos:prefLabel "catch"@en ;
    skos:related swift:DoCatch .

swift:convenience a owl:NamedIndividual,
        skos:Concept ;
    skos:broader swift:Keyword ;
    skos:inScheme swift:Scheme ;
    skos:prefLabel "convenience"@en ;
    skos:related swift:ConvenienceInitializer .

swift:defer a owl:NamedIndividual,
        skos:Concept ;
    skos:broader swift:Keyword ;
    skos:definition <https://docs.swift.org/swift-book/LanguageGuide/ErrorHandling.html#ID514> ;
    skos:inScheme swift:Scheme ;
    skos:prefLabel "defer"@en ;
    skos:related swift:ErrorHandling .

swift:deinit a owl:NamedIndividual,
        skos:Concept ;
    skos:broader swift:Keyword ;
    skos:inScheme swift:Scheme ;
    skos:prefLabel "deinit"@en ;
    skos:related swift:Deinitializer .

swift:do a owl:NamedIndividual,
        skos:Concept ;
    skos:broader swift:Keyword ;
    skos:inScheme swift:Scheme ;
    skos:prefLabel "do"@en ;
    skos:related swift:DoCatch .

swift:enum a owl:NamedIndividual,
        skos:Concept ;
    skos:broader swift:Keyword ;
    skos:inScheme swift:Scheme ;
    skos:prefLabel "enum"@en ;
    skos:related swift:Enumeration .

swift:fallthrough a owl:NamedIndividual,
        skos:Concept ;
    skos:broader swift:Keyword ;
    skos:definition <https://docs.swift.org/swift-book/LanguageGuide/ControlFlow.html#ID140> ;
    skos:inScheme swift:Scheme ;
    skos:prefLabel "fallthrough"@en ;
    skos:related swift:ControlFlow,
        swift:Switch .

swift:fileprivate a owl:NamedIndividual,
        skos:Concept ;
    skos:broader swift:Keyword ;
    skos:inScheme swift:Scheme ;
    skos:prefLabel "fileprivate"@en ;
    skos:related swift:FilePrivateAccess .

swift:final a owl:NamedIndividual,
        skos:Concept ;
    skos:broader swift:Keyword ;
    skos:definition <https://docs.swift.org/swift-book/LanguageGuide/Inheritance.html#ID202> ;
    skos:inScheme swift:Scheme ;
    skos:prefLabel "final"@en ;
    skos:related swift:Overriding .

swift:func a owl:NamedIndividual,
        skos:Concept ;
    skos:broader swift:Keyword ;
    skos:inScheme swift:Scheme ;
    skos:prefLabel "func"@en ;
    skos:related swift:Function .

swift:import a owl:NamedIndividual,
        skos:Concept ;
    skos:broader swift:Keyword ;
    skos:inScheme swift:Scheme ;
    skos:prefLabel "import"@en ;
    skos:related swift:Module .

swift:init a owl:NamedIndividual,
        skos:Concept ;
    skos:broader swift:Keyword ;
    skos:inScheme swift:Scheme ;
    skos:prefLabel "init"@en ;
    skos:related swift:Initializer .

swift:inout a owl:NamedIndividual,
        skos:Concept ;
    skos:broader swift:Keyword ;
    skos:inScheme swift:Scheme ;
    skos:prefLabel "inout"@en ;
    skos:related swift:InOutParameter .

swift:internal a owl:NamedIndividual,
        skos:Concept ;
    skos:broader swift:Keyword ;
    skos:inScheme swift:Scheme ;
    skos:prefLabel "internal"@en ;
    skos:related swift:InternalAccess .

swift:is a owl:NamedIndividual,
        skos:Concept ;
    skos:broader swift:Keyword ;
    skos:inScheme swift:Scheme ;
    skos:prefLabel "is"@en ;
    skos:related swift:TypeCheckOperator .

swift:let a owl:NamedIndividual,
        skos:Concept ;
    skos:broader swift:Keyword ;
    skos:inScheme swift:Scheme ;
    skos:prefLabel "let"@en ;
    skos:related swift:Constant .

swift:mutating a owl:NamedIndividual,
        skos:Concept ;
    skos:broader swift:Keyword ;
    skos:definition <https://docs.swift.org/swift-book/LanguageGuide/Methods.html#ID239> ;
    skos:inScheme swift:Scheme ;
    skos:prefLabel "mutating"@en ;
    skos:related swift:Instance,
        swift:Method,
        swift:ValueType .

swift:nil a owl:NamedIndividual,
        skos:Concept ;
    skos:inScheme swift:Scheme ;
    skos:prefLabel "nil"@en ;
    skos:related dbr:Null_pointer,
        swift:Optional .

swift:override a owl:NamedIndividual,
        skos:Concept ;
    skos:broader swift:Keyword ;
    skos:inScheme swift:Scheme ;
    skos:prefLabel "override"@en ;
    skos:related swift:Overriding .

swift:print a owl:NamedIndividual,
        skos:Concept ;
    skos:broader swift:Function ;
    skos:definition <https://docs.swift.org/swift-book/LanguageGuide/TheBasics.html#ID314> ;
    skos:inScheme swift:Scheme ;
    skos:prefLabel "print"@en ;
    skos:related dbr:Printf_format_string .

swift:private a owl:NamedIndividual,
        skos:Concept ;
    skos:broader swift:Keyword ;
    skos:inScheme swift:Scheme ;
    skos:prefLabel "private"@en ;
    skos:related swift:PrivateAccess .

swift:public a owl:NamedIndividual,
        skos:Concept ;
    skos:broader swift:Keyword ;
    skos:inScheme swift:Scheme ;
    skos:prefLabel "public"@en ;
    skos:related swift:PublicAccess .

swift:required a owl:NamedIndividual,
        skos:Concept ;
    skos:broader swift:Keyword ;
    skos:inScheme swift:Scheme ;
    skos:prefLabel "required"@en ;
    skos:related swift:RequiredInitializer .

swift:return a owl:NamedIndividual,
        skos:Concept ;
    skos:broader swift:Keyword ;
    skos:definition <https://docs.swift.org/swift-book/LanguageGuide/Functions.html#ID160> ;
    skos:inScheme swift:Scheme ;
    skos:prefLabel "return"@en ;
    skos:related dbr:Return_statement,
        swift:ControlFlow,
        swift:ReturnValue .

swift:self a owl:NamedIndividual,
        skos:Concept ;
    skos:broader swift:Keyword ;
    skos:definition <https://docs.swift.org/swift-book/LanguageGuide/Methods.html#ID238> ;
    skos:inScheme swift:Scheme ;
    skos:prefLabel "self"@en ;
    skos:related dbr:This_%28computer_programming%29,
        swift:Instance,
        swift:Method .

swift:some a owl:NamedIndividual,
        skos:Concept ;
    skos:broader swift:Keyword ;
    skos:inScheme swift:Scheme ;
    skos:prefLabel "some"@en ;
    skos:related swift:OpaqueType .

swift:super a owl:NamedIndividual,
        skos:Concept ;
    skos:broader swift:Keyword ;
    skos:definition <https://docs.swift.org/swift-book/ReferenceManual/Expressions.html#ID392> ;
    skos:inScheme swift:Scheme ;
    skos:prefLabel "super"@en ;
    skos:related swift:BaseClass .

swift:throw a owl:NamedIndividual,
        skos:Concept ;
    skos:broader swift:Keyword ;
    skos:definition <https://docs.swift.org/swift-book/LanguageGuide/ErrorHandling.html#ID509> ;
    skos:inScheme swift:Scheme ;
    skos:prefLabel "throw"@en ;
    skos:related swift:ControlFlow,
        swift:ErrorHandling .

swift:throws a owl:NamedIndividual,
        skos:Concept ;
    skos:broader swift:Keyword ;
    skos:definition <https://docs.swift.org/swift-book/LanguageGuide/ErrorHandling.html#ID510> ;
    skos:inScheme swift:Scheme ;
    skos:prefLabel "throws"@en ;
    skos:related swift:ErrorHandling,
        swift:Function .

swift:try a owl:NamedIndividual,
        skos:Concept ;
    skos:broader swift:Keyword ;
    skos:inScheme swift:Scheme ;
    skos:prefLabel "try"@en ;
    skos:related swift:ErrorHandling .

swift:unowned a owl:NamedIndividual,
        skos:Concept ;
    skos:broader swift:Keyword ;
    skos:inScheme swift:Scheme ;
    skos:prefLabel "unowned"@en ;
    skos:related swift:UnownedReference .

swift:var a owl:NamedIndividual,
        skos:Concept ;
    skos:broader swift:Keyword ;
    skos:inScheme swift:Scheme ;
    skos:prefLabel "var"@en ;
    skos:related swift:Variable .

swift:weak a owl:NamedIndividual,
        skos:Concept ;
    skos:broader swift:Keyword ;
    skos:inScheme swift:Scheme ;
    skos:prefLabel "weak"@en ;
    skos:related swift:WeakReference .

swift:where a owl:NamedIndividual,
        skos:Concept ;
    skos:broader swift:Keyword ;
    skos:definition <https://docs.swift.org/swift-book/LanguageGuide/ControlFlow.html#ID134> ;
    skos:inScheme swift:Scheme ;
    skos:prefLabel "where"@en ;
    skos:related swift:GenericWhereClause .

swift:AssignmentOperator a owl:NamedIndividual,
        skos:Concept ;
    skos:broader swift:Operator ;
    skos:definition <https://docs.swift.org/swift-book/LanguageGuide/BasicOperators.html#ID62> ;
    skos:inScheme swift:Scheme ;
    skos:prefLabel "Assignment Operator"@en ;
    skos:related dbr:Assignment_%28computer_science%29,
        dbr:Operator_%28computer_programming%29 .

swift:BaseClass a owl:NamedIndividual,
        skos:Concept ;
    skos:definition <https://docs.swift.org/swift-book/LanguageGuide/Inheritance.html#ID194> ;
    skos:inScheme swift:Scheme ;
    skos:prefLabel "Base Class"@en ;
    skos:related dbr:Superclass_%28computer_science%29,
        swift:Inheritance .

swift:ComputedProperty a owl:NamedIndividual,
        skos:Concept ;
    skos:broader swift:Property ;
    skos:definition <https://docs.swift.org/swift-book/LanguageGuide/Properties.html#ID259> ;
    skos:inScheme swift:Scheme ;
    skos:prefLabel "Computed Property"@en ;
    skos:related dbr:Property_%28programming%29 .

swift:Constant a owl:NamedIndividual,
        skos:Concept ;
    skos:definition <https://docs.swift.org/swift-book/LanguageGuide/TheBasics.html#ID310> ;
    skos:inScheme swift:Scheme ;
    skos:prefLabel "Constant"@en ;
    skos:related dbr:Constant_%28computer_programming%29 .

swift:ConvenienceInitializer a owl:NamedIndividual,
        skos:Concept ;
    skos:broader swift:Initializer ;
    skos:definition <https://docs.swift.org/swift-book/LanguageGuide/Initialization.html#ID217> ;
    skos:inScheme swift:Scheme ;
    skos:prefLabel "Convenience Initializer"@en .

swift:Deinitializer a owl:NamedIndividual,
        skos:Concept ;
    skos:definition <https://docs.swift.org/swift-book/LanguageGuide/Deinitialization.html#deinitialization> ;
    skos:inScheme swift:Scheme ;
    skos:prefLabel "Deinitializer"@en ;
    skos:related dbr:Destructor_%28computer_programming%29 .

swift:DownCasting a owl:NamedIndividual,
        skos:Concept ;
    skos:broader swift:TypeCasting ;
    skos:definition <https://docs.swift.org/swift-book/LanguageGuide/TypeCasting.html#ID341> ;
    skos:inScheme swift:Scheme ;
    skos:prefLabel "Downcasting"@en ;
    skos:related dbr:Downcasting .

swift:Extension a owl:NamedIndividual,
        skos:Concept ;
    skos:definition <https://docs.swift.org/swift-book/LanguageGuide/Extensions.html#extensions> ;
    skos:inScheme swift:Scheme ;
    skos:prefLabel "Extension"@en ;
    skos:related swift:Class,
        swift:Enumeration,
        swift:Protocol,
        swift:Struct .

swift:FilePrivateAccess a owl:NamedIndividual,
        skos:Concept ;
    skos:broader swift:AccessLevel ;
    skos:inScheme swift:Scheme ;
    skos:prefLabel "File-private Access"@en .

swift:GenericWhereClause a owl:NamedIndividual,
        skos:Concept ;
    skos:definition <https://docs.swift.org/swift-book/LanguageGuide/Generics.html#ID192> ;
    skos:inScheme swift:Scheme ;
    skos:prefLabel "Generic Where Clause"@en ;
    skos:related swift:GenericType,
        swift:TypeConstraint .

swift:InOutParameter a owl:NamedIndividual,
        skos:Concept ;
    skos:broader swift:Parameter ;
    skos:definition <https://docs.swift.org/swift-book/LanguageGuide/Functions.html#ID173> ;
    skos:inScheme swift:Scheme ;
    skos:prefLabel "In-Out Parameter"@en ;
    skos:related dbr:Evaluation_strategy .

swift:InternalAccess a owl:NamedIndividual,
        skos:Concept ;
    skos:broader swift:AccessLevel ;
    skos:inScheme swift:Scheme ;
    skos:prefLabel "Internal Access"@en .

swift:MethodRequirement a owl:NamedIndividual,
        skos:Concept ;
    skos:definition <https://docs.swift.org/swift-book/LanguageGuide/Protocols.html#ID270> ;
    skos:inScheme swift:Scheme ;
    skos:prefLabel "Method Requirement"@en ;
    skos:related dbr:Abstract_type,
        swift:Method,
        swift:Protocol .

swift:Module a owl:NamedIndividual,
        skos:Concept ;
    skos:definition <https://docs.swift.org/swift-book/LanguageGuide/AccessControl.html#ID4> ;
    skos:inScheme swift:Scheme ;
    skos:prefLabel "Module"@en ;
    skos:related dbr:Modular_programming,
        swift:AccessControl .

swift:OpaqueType a owl:NamedIndividual,
        skos:Concept ;
    skos:broader swift:Type ;
    skos:definition <https://docs.swift.org/swift-book/LanguageGuide/OpaqueTypes.html#opaque-types> ;
    skos:inScheme swift:Scheme ;
    skos:prefLabel "Opaque Type"@en ;
    skos:related swift:ReturnValue .

swift:OperatorMethod a owl:NamedIndividual,
        skos:Concept ;
    skos:broader swift:Operator ;
    skos:definition <https://docs.swift.org/swift-book/LanguageGuide/AdvancedOperators.html#ID42> ;
    skos:inScheme swift:Scheme ;
    skos:prefLabel "Operator Method"@en ;
    skos:related swift:Method .

swift:PrivateAccess a owl:NamedIndividual,
        skos:Concept ;
    skos:broader swift:AccessLevel ;
    skos:inScheme swift:Scheme ;
    skos:prefLabel "Private Access"@en .

swift:PropertyRequirement a owl:NamedIndividual,
        skos:Concept ;
    skos:definition <https://docs.swift.org/swift-book/LanguageGuide/Protocols.html#ID269> ;
    skos:inScheme swift:Scheme ;
    skos:prefLabel "Property Requirement"@en ;
    skos:related swift:Property,
        swift:Protocol .

swift:PublicAccess a owl:NamedIndividual,
        skos:Concept ;
    skos:broader swift:AccessLevel ;
    skos:inScheme swift:Scheme ;
    skos:prefLabel "Public Access"@en .

swift:RequiredInitializer a owl:NamedIndividual,
        skos:Concept ;
    skos:broader swift:Initializer ;
    skos:definition <https://docs.swift.org/swift-book/LanguageGuide/Initialization.html#ID231> ;
    skos:inScheme swift:Scheme ;
    skos:prefLabel "Required Initializer"@en .

swift:StoredProperty a owl:NamedIndividual,
        skos:Concept ;
    skos:broader swift:Property ;
    skos:definition <https://docs.swift.org/swift-book/LanguageGuide/Properties.html#ID255> ;
    skos:inScheme swift:Scheme ;
    skos:prefLabel "Stored Property"@en ;
    skos:related dbr:Field_%28computer_science%29 .

swift:String a owl:NamedIndividual,
        skos:Concept ;
    skos:broader swift:Struct ;
    skos:definition <https://docs.swift.org/swift-book/LanguageGuide/StringsAndCharacters.html> ;
    skos:inScheme swift:Scheme ;
    skos:prefLabel "String"@en ;
    skos:related dbr:String_%28computer_science%29 .

swift:Subscript a owl:NamedIndividual,
        skos:Concept ;
    skos:broader swift:ComputedProperty ;
    skos:definition <https://docs.swift.org/swift-book/LanguageGuide/Subscripts.html#subscripts> ;
    skos:inScheme swift:Scheme ;
    skos:prefLabel "Subscript"@en ;
    skos:related dbr:Index_notation,
        swift:Class,
        swift:Enumeration,
        swift:Struct .

swift:TypeCheckOperator a owl:NamedIndividual,
        skos:Concept ;
    skos:broader swift:Operator,
        swift:TypeCasting ;
    skos:definition <https://docs.swift.org/swift-book/LanguageGuide/TypeCasting.html#ID340> ;
    skos:inScheme swift:Scheme ;
    skos:prefLabel "Type Check Operator"@en ;
    skos:related dbr:Type_introspection .

swift:TypeConstraint a owl:NamedIndividual,
        skos:Concept ;
    skos:definition <https://docs.swift.org/swift-book/LanguageGuide/Generics.html#ID186> ;
    skos:inScheme swift:Scheme ;
    skos:prefLabel "Type Constraint"@en ;
    skos:related dbr:Bounded_quantification,
        swift:GenericType .

swift:UnownedReference a owl:NamedIndividual,
        skos:Concept ;
    skos:definition <https://docs.swift.org/swift-book/LanguageGuide/AutomaticReferenceCounting.html#ID54> ;
    skos:inScheme swift:Scheme ;
    skos:prefLabel "Unowned Reference"@en ;
    skos:related swift:ARC .

swift:Variable a owl:NamedIndividual,
        skos:Concept ;
    skos:definition <https://docs.swift.org/swift-book/LanguageGuide/TheBasics.html#ID310> ;
    skos:inScheme swift:Scheme ;
    skos:prefLabel "Variable"@en ;
    skos:related dbr:Variable_%28computer_science%29 .

swift:WeakReference a owl:NamedIndividual,
        skos:Concept ;
    skos:definition <https://docs.swift.org/swift-book/LanguageGuide/AutomaticReferenceCounting.html#ID53> ;
    skos:inScheme swift:Scheme ;
    skos:prefLabel "Weak Reference"@en ;
    skos:related dbr:Weak_reference,
        swift:ARC .

swift:break a owl:NamedIndividual,
        skos:Concept ;
    skos:broader swift:Keyword ;
    skos:definition <https://docs.swift.org/swift-book/LanguageGuide/ControlFlow.html#ID137> ;
    skos:inScheme swift:Scheme ;
    skos:prefLabel "break"@en ;
    skos:related dbr:Control_flow,
        swift:ControlFlow .

swift:continue a owl:NamedIndividual,
        skos:Concept ;
    skos:broader swift:Keyword ;
    skos:definition <https://docs.swift.org/swift-book/LanguageGuide/ControlFlow.html#ID136> ;
    skos:inScheme swift:Scheme ;
    skos:prefLabel "continue"@en ;
    skos:related dbr:Control_flow,
        swift:ControlFlow .

swift:AccessControl a owl:NamedIndividual,
        skos:Concept ;
    skos:definition <https://docs.swift.org/swift-book/LanguageGuide/AccessControl.html#access-control> ;
    skos:inScheme swift:Scheme ;
    skos:prefLabel "Access Control"@en ;
    skos:related dbr:Encapsulation_%28computer_programming%29 .

swift:DoCatch a owl:NamedIndividual,
        skos:Concept ;
    skos:definition <https://docs.swift.org/swift-book/LanguageGuide/ErrorHandling.html#ID541> ;
    skos:inScheme swift:Scheme ;
    skos:prefLabel "Do-Catch"@en ;
    skos:related swift:ErrorHandling .

swift:Generics a owl:NamedIndividual,
        skos:Concept ;
    skos:definition <https://docs.swift.org/swift-book/LanguageGuide/Generics.html#generics> ;
    skos:inScheme swift:Scheme ;
    skos:prefLabel "Generics"@en ;
    skos:related dbr:Generic_programming .

swift:If a owl:NamedIndividual,
        skos:Concept ;
    skos:broader swift:ConditionalStatement ;
    skos:definition <https://docs.swift.org/swift-book/LanguageGuide/ControlFlow.html#ID128> ;
    skos:inScheme swift:Scheme ;
    skos:prefLabel "If"@en ;
    skos:related dbr:Conditional_%28computer_programming%29,
        dbr:Control_flow .

swift:Instance a owl:NamedIndividual,
        skos:Concept ;
    skos:definition <https://docs.swift.org/swift-book/LanguageGuide/ClassesAndStructures.html#ID85> ;
    skos:inScheme swift:Scheme ;
    skos:prefLabel "Instance"@en ;
    skos:related dbr:Object_%28computer_science%29,
        swift:Class,
        swift:Struct .

swift:Overriding a owl:NamedIndividual,
        skos:Concept ;
    skos:definition <https://docs.swift.org/swift-book/LanguageGuide/Inheritance.html#ID196> ;
    skos:inScheme swift:Scheme ;
    skos:prefLabel "Overriding"@en ;
    skos:related dbr:Method_overriding,
        swift:Inheritance .

swift:ReturnValue a owl:NamedIndividual,
        skos:Concept ;
    skos:definition <https://docs.swift.org/swift-book/LanguageGuide/Functions.html#ID160> ;
    skos:inScheme swift:Scheme ;
    skos:prefLabel "Return Value"@en ;
    skos:related dbr:Return_type,
        swift:Function .

swift:Switch a owl:NamedIndividual,
        skos:Concept ;
    skos:broader swift:ConditionalStatement ;
    skos:definition <https://docs.swift.org/swift-book/LanguageGuide/ControlFlow.html#ID129> ;
    skos:inScheme swift:Scheme ;
    skos:prefLabel "Switch"@en ;
    skos:related dbr:Switch_statement .

swift:ARC a owl:NamedIndividual,
        skos:Concept ;
    skos:definition <https://docs.swift.org/swift-book/LanguageGuide/AutomaticReferenceCounting.html#automatic-reference-counting> ;
    skos:inScheme swift:Scheme ;
    skos:prefLabel "Automatic Reference Counting"@en ;
    skos:related dbr:Automatic_Reference_Counting .

swift:Collection a owl:NamedIndividual,
        skos:Concept ;
    skos:broader swift:Struct ;
    skos:definition <https://docs.swift.org/swift-book/LanguageGuide/CollectionTypes.html> ;
    skos:inScheme swift:Scheme ;
    skos:prefLabel "Collection"@en ;
    skos:related dbr:Collection_%28abstract_data_type%29 .

swift:ConditionalStatement a owl:NamedIndividual,
        skos:Concept ;
    skos:broader swift:ControlFlow ;
    skos:definition <https://docs.swift.org/swift-book/LanguageGuide/ControlFlow.html#ID127> ;
    skos:inScheme swift:Scheme ;
    skos:prefLabel "Conditional Statement"@en ;
    skos:related dbr:Conditional_%28computer_programming%29 .

swift:Inheritance a owl:NamedIndividual,
        skos:Concept ;
    skos:definition <https://docs.swift.org/swift-book/LanguageGuide/Inheritance.html#inheritance> ;
    skos:inScheme swift:Scheme ;
    skos:prefLabel "Inheritance"@en ;
    skos:related dbr:Inheritance_%28object-oriented_programming%29,
        swift:Class .

swift:Loop a owl:NamedIndividual,
        skos:Concept ;
    skos:broader swift:ControlFlow ;
    skos:inScheme swift:Scheme ;
    skos:prefLabel "Loop"@en ;
    skos:related dbr:Control_flow .

swift:Closure a owl:NamedIndividual,
        skos:Concept ;
    skos:broader swift:ReferenceType ;
    skos:definition <https://docs.swift.org/swift-book/LanguageGuide/Closures.html> ;
    skos:inScheme swift:Scheme ;
    skos:prefLabel "Closure"@en ;
    skos:related dbr:Closure_%28computer_programming%29 .

swift:GenericType a owl:NamedIndividual,
        skos:Concept ;
    skos:broader swift:Type ;
    skos:definition <https://docs.swift.org/swift-book/LanguageGuide/Generics.html#ID184> ;
    skos:inScheme swift:Scheme ;
    skos:prefLabel "Generic Type"@en ;
    skos:related dbr:Generic_programming,
        dbr:Generics_in_Java,
        swift:Generics .

swift:ReferenceType a owl:NamedIndividual,
        skos:Concept ;
    skos:broader swift:Type ;
    skos:definition <https://docs.swift.org/swift-book/LanguageGuide/ClassesAndStructures.html#ID89> ;
    skos:inScheme swift:Scheme ;
    skos:prefLabel "Reference Type"@en ;
    skos:related dbr:Reference_type .

swift:TypeCasting a owl:NamedIndividual,
        skos:Concept ;
    skos:definition <https://docs.swift.org/swift-book/LanguageGuide/TypeCasting.html#type-casting> ;
    skos:inScheme swift:Scheme ;
    skos:prefLabel "Type Casting"@en ;
    skos:related dbr:Type_conversion,
        swift:Type .

swift:ValueType a owl:NamedIndividual,
        skos:Concept ;
    skos:broader swift:Type ;
    skos:definition <https://docs.swift.org/swift-book/LanguageGuide/ClassesAndStructures.html#ID88> ;
    skos:inScheme swift:Scheme ;
    skos:prefLabel "Value Type"@en ;
    skos:related dbr:Value_type .

swift:AccessLevel a owl:NamedIndividual,
        skos:Concept ;
    skos:broader swift:AccessControl ;
    skos:definition <https://docs.swift.org/swift-book/LanguageGuide/AccessControl.html#ID5> ;
    skos:inScheme swift:Scheme ;
    skos:prefLabel "Access Level"@en ;
    skos:related dbr:Access_level .

swift:ErrorHandling a owl:NamedIndividual,
        skos:Concept ;
    skos:definition <https://docs.swift.org/swift-book/LanguageGuide/ErrorHandling.html#error-handling> ;
    skos:inScheme swift:Scheme ;
    skos:prefLabel "Error Handling"@en ;
    skos:related dbr:Exception_handling .

swift:Optional a owl:NamedIndividual,
        skos:Concept ;
    skos:broader swift:Type ;
    skos:definition <https://docs.swift.org/swift-book/LanguageGuide/TheBasics.html#ID330> ;
    skos:inScheme swift:Scheme ;
    skos:prefLabel "Optional"@en ;
    skos:related dbr:Option_type .

swift:Parameter a owl:NamedIndividual,
        skos:Concept ;
    skos:definition <https://docs.swift.org/swift-book/LanguageGuide/Functions.html#ID160> ;
    skos:inScheme swift:Scheme ;
    skos:prefLabel "Parameter"@en ;
    skos:related dbr:Parameter_%28computer_programming%29,
        swift:Function .

swift:Method a owl:NamedIndividual,
        skos:Concept ;
    skos:broader swift:Function ;
    skos:definition <https://docs.swift.org/swift-book/LanguageGuide/Methods.html#methods> ;
    skos:inScheme swift:Scheme ;
    skos:prefLabel "Method"@en ;
    skos:related dbr:Method_%28computer_programming%29,
        swift:Class,
        swift:Enumeration,
        swift:Struct .

swift:Property a owl:NamedIndividual,
        skos:Concept ;
    skos:definition <https://docs.swift.org/swift-book/LanguageGuide/Properties.html#properties> ;
    skos:inScheme swift:Scheme ;
    skos:prefLabel "Property"@en ;
    skos:related dbr:Property_%28programming%29,
        swift:Class,
        swift:Enumeration,
        swift:Struct .

swift:Protocol a owl:NamedIndividual,
        skos:Concept ;
    skos:broader swift:Type ;
    skos:definition <https://docs.swift.org/swift-book/LanguageGuide/Protocols.html#protocols> ;
    skos:inScheme swift:Scheme ;
    skos:prefLabel "Protocol"@en ;
    skos:related dbr:Interface_%28Java%29,
        dbr:Protocol_%28object-oriented_programming%29 .

swift:Class a owl:NamedIndividual,
        skos:Concept ;
    skos:broader swift:ReferenceType ;
    skos:definition <https://docs.swift.org/swift-book/LanguageGuide/ClassesAndStructures.html#structures-and-classes> ;
    skos:inScheme swift:Scheme ;
    skos:prefLabel "Class"@en ;
    skos:related dbr:Class_%28computer_programming%29 .

swift:ControlFlow a owl:NamedIndividual,
        skos:Concept ;
    skos:definition <https://docs.swift.org/swift-book/LanguageGuide/ControlFlow.html#control-flow> ;
    skos:inScheme swift:Scheme ;
    skos:prefLabel "Control Flow"@en ;
    skos:related dbr:Control_flow .

swift:Function a owl:NamedIndividual,
        skos:Concept ;
    skos:broader swift:ReferenceType ;
    skos:definition <https://docs.swift.org/swift-book/LanguageGuide/Functions.html> ;
    skos:inScheme swift:Scheme ;
    skos:prefLabel "Function"@en ;
    skos:related dbr:Subroutine .

swift:Initializer a owl:NamedIndividual,
        skos:Concept ;
    skos:broader swift:Method ;
    skos:definition <https://docs.swift.org/swift-book/LanguageGuide/Initialization.html#ID205> ;
    skos:inScheme swift:Scheme ;
    skos:prefLabel "Initializer"@en ;
    skos:related dbr:Constructor_%28object-oriented_programming%29,
        swift:Class,
        swift:Enumeration,
        swift:Struct .

swift:Enumeration a owl:NamedIndividual,
        skos:Concept ;
    skos:broader swift:ValueType ;
    skos:definition <https://docs.swift.org/swift-book/LanguageGuide/Enumerations.html#enumerations> ;
    skos:inScheme swift:Scheme ;
    skos:prefLabel "Enumeration"@en ;
    skos:related dbr:Enumerated_type .

swift:Struct a owl:NamedIndividual,
        skos:Concept ;
    skos:broader swift:ValueType ;
    skos:definition <https://docs.swift.org/swift-book/LanguageGuide/ClassesAndStructures.html#structures-and-classes> ;
    skos:inScheme swift:Scheme ;
    skos:prefLabel "Struct"@en ;
    skos:related dbr:Record_%28computer_science%29 .

swift:Operator a owl:NamedIndividual,
        skos:Concept ;
    skos:definition <https://docs.swift.org/swift-book/LanguageGuide/BasicOperators.html#basic-operators> ;
    skos:inScheme swift:Scheme ;
    skos:prefLabel "Operator"@en ;
    skos:related dbr:Operator_%28computer_programming%29 .

swift:Type a owl:NamedIndividual,
        skos:Concept ;
    skos:definition <https://docs.swift.org/swift-book/ReferenceManual/Types.html#types> ;
    skos:inScheme swift:Scheme ;
    skos:prefLabel "Type"@en ;
    skos:related dbr:Data_type .

swift:Keyword a owl:NamedIndividual,
        skos:Concept ;
    skos:definition <https://docs.swift.org/swift-book/ReferenceManual/LexicalStructure.html#ID413> ;
    skos:inScheme swift:Scheme ;
    skos:prefLabel "Keyword"@en ;
    skos:related dbr:Keyword_%28computer_programming%29 .

swift:Scheme a skos:ConceptScheme ;
    dct:title "Swift" ;
    skos:hasTopConcept swift:ARC,
        swift:AccessControl,
        swift:ArgumentLabel,
        swift:AssociatedType,
        swift:AssociatedValue,
        swift:Attribute,
        swift:BaseClass,
        swift:Comment,
        swift:CompilerControlStatement,
        swift:Constant,
        swift:ControlFlow,
        swift:DefaultParameterValue,
        swift:DefaultPropertyValue,
        swift:Deinitializer,
        swift:DoCatch,
        swift:ErrorHandling,
        swift:Extension,
        swift:ForcedUnwrapping,
        swift:GenericWhereClause,
        swift:Generics,
        swift:Inheritance,
        swift:InitializerDelegation,
        swift:InitializerRequirement,
        swift:Instance,
        swift:Keyword,
        swift:MethodRequirement,
        swift:Module,
        swift:Operator,
        swift:OptionalBinding,
        swift:OptionalChaining,
        swift:OptionalProtocolRequirement,
        swift:Overriding,
        swift:Parameter,
        swift:Property,
        swift:PropertyObserver,
        swift:PropertyRequirement,
        swift:PropertyWrapper,
        swift:RawValue,
        swift:ReturnValue,
        swift:StringInterpolation,
        swift:StrongReference,
        swift:Subclassing,
        swift:Type,
        swift:TypeAlias,
        swift:TypeAnnotation,
        swift:TypeCasting,
        swift:TypeConstraint,
        swift:TypeInference,
        swift:UnownedReference,
        swift:Variable,
        swift:WeakReference,
        swift:nil .
